Implemented Arrays.replace1with2

lib/Arrays.dfy
@@ -39,6 +39,23 @@ module Arrays {
     }
   }
 
+  method replace1with2<T>(arr: array<T>, length: uint64, element1: T, element2: T, pos: uint64)
+    requires 0 <= length as int < arr.Length < Uint64UpperBound()
+    requires 0 <= pos < length
+    ensures arr[..length+1] == Seq.replace1with2(old(arr[..length]), element1, element2, pos as int)
+    ensures arr[length+1..] == old(arr[length+1..])
+    modifies arr
+  {
+    Insert(arr, length, element2, pos+1);
+    arr[pos] := element1;
+
+    ghost var replaced := Seq.replace1with2(old(arr[..length]), element1, element2, pos as int);
+    assert forall i :: 0 <= i < pos ==> arr[i] == replaced[i];
+    assert arr[pos] == replaced[pos];
+    assert arr[pos+1] == replaced[pos+1];
+    assert forall i :: pos+2 <= i < length+1 ==> arr[i] == old(arr[i-1]);
+  }
+  
   method Memcpy<T>(dest: array<T>, destoffset: uint64, src: seq<T>)
     requires 0 <= destoffset as int <= dest.Length - |src|
     ensures dest[..] == old(dest[..destoffset]) + src + old(dest[destoffset as int + |src|..])
